Change Locmap to map locations to encoded bytes
Instead of mapping locations to values directly, map them to lists of
encoded bytes (`list memval`). Locmap accesses must now pass through
encoding and decoding steps. The new `ls @ l` notation wraps read access
(i.e., `Locmap.get`) to locset `ls` at location `l`.

As a side effect, as read accesses `ls @ l` involve a decoding step
involving the type of the location `l`, the result read always has the type
of `l`. The notion of a well-typed locset, used in LTL and Linear semantics,
becomes trivial: All locsets are now well-typed. This simplifies some proofs
in Lineartyping and LTLtyping. A future patch can simplify things further.

backend/Allocproof.v
@@ -433,7 +433,7 @@ Definition sel_val (k: equation_kind) (v: val) : val :=
   is less defined than [ls l] (the value of [l] in the LTL code). *)
 
 Definition satisf (rs: regset) (ls: locset) (e: eqs) : Prop :=
-  forall q, EqSet.In q e -> Val.lessdef (sel_val (ekind q) rs#(ereg q)) (ls (eloc q)).
+  forall q, EqSet.In q e -> Val.lessdef (sel_val (ekind q) rs#(ereg q)) (ls @ (eloc q)).
 
 Lemma empty_eqs_satisf:
   forall rs ls, satisf rs ls empty_eqs.
@@ -459,7 +459,7 @@ Qed.
 
 Lemma add_equation_lessdef:
   forall rs ls q e,
-  satisf rs ls (add_equation q e) -> Val.lessdef (sel_val (ekind q) rs#(ereg q)) (ls (eloc q)).
+  satisf rs ls (add_equation q e) -> Val.lessdef (sel_val (ekind q) rs#(ereg q)) (ls @ (eloc q)).
 Proof.
   intros. apply H. unfold add_equation. simpl. apply EqSet.add_1. auto.
 Qed.
@@ -1075,9 +1075,9 @@ Lemma subst_loc_satisf:
   subst_loc dst src e = Some e' ->
   loc_type_compat env dst e = true ->
   wt_regset env rs ->
-  Val.has_type (ls src) (Loc.type dst) ->
+  Val.has_type (ls @ src) (Loc.type dst) ->
   satisf rs ls e' ->
-  satisf rs (Locmap.set dst (ls src) ls) e.
+  satisf rs (Locmap.set dst (ls @ src) ls) e.
 Proof.
   intros; red; intros.
   exploit in_subst_loc; eauto. intros [[A B] | [A B]].
@@ -1139,9 +1139,9 @@ Qed.
 Lemma subst_loc_part_satisf_lowlong:
   forall src dst rs ls e e',
   subst_loc_part (R dst) (R src) Low e = Some e' ->
-  Val.has_type (Val.loword (ls (R src))) (mreg_type dst) ->
+  Val.has_type (Val.loword (ls @ (R src))) (mreg_type dst) ->
   satisf rs ls e' ->
-  satisf rs (Locmap.set (R dst) (Val.loword (ls (R src))) ls) e.
+  satisf rs (Locmap.set (R dst) (Val.loword (ls @ (R src))) ls) e.
 Proof.
   intros; red; intros.
   exploit in_subst_loc_part; eauto. intros [[A [B C]] | [A B]].
@@ -1153,9 +1153,9 @@ Qed.
 Lemma subst_loc_part_satisf_highlong:
   forall src dst rs ls e e',
   subst_loc_part (R dst) (R src) High e = Some e' ->
-  Val.has_type (Val.hiword (ls (R src))) (mreg_type dst) ->
+  Val.has_type (Val.hiword (ls @ (R src))) (mreg_type dst) ->
   satisf rs ls e' ->
-  satisf rs (Locmap.set (R dst) (Val.hiword (ls (R src))) ls) e.
+  satisf rs (Locmap.set (R dst) (Val.hiword (ls @ (R src))) ls) e.
 Proof.
   intros; red; intros.
   exploit in_subst_loc_part; eauto. intros [[A [B C]] | [A B]].
@@ -1242,8 +1242,8 @@ Lemma subst_loc_pair_satisf_makelong:
   wt_regset env rs ->
   satisf rs ls e' ->
   Archi.ptr64 = false ->
-  Val.has_type (Val.longofwords (ls (R src1)) (ls (R src2))) (mreg_type dst) ->
-  satisf rs (Locmap.set (R dst) (Val.longofwords (ls (R src1)) (ls (R src2))) ls) e.
+  Val.has_type (Val.longofwords (ls @ (R src1)) (ls @ (R src2))) (mreg_type dst) ->
+  satisf rs (Locmap.set (R dst) (Val.longofwords (ls @ (R src1)) (ls @ (R src2))) ls) e.
 Proof.
   intros; red; intros.
   exploit in_subst_loc_pair; eauto. intros [[A [B [C D]]] | [A B]].
@@ -1272,7 +1272,7 @@ Qed.
 
 Lemma undef_regs_outside:
   forall ml ls l,
-  Loc.notin l (map R ml) -> undef_regs ml ls l = ls l.
+  Loc.notin l (map R ml) -> (undef_regs ml ls) @ l = ls @ l.
 Proof.
   induction ml; simpl; intros. auto.
   rewrite Locmap.gso. apply IHml. tauto. apply Loc.diff_sym. tauto.
@@ -1308,7 +1308,7 @@ Lemma subst_loc_undef_satisf:
   can_undef_except dst ml e = true ->
   wt_regset env rs ->
   satisf rs ls e' ->
-  satisf rs (Locmap.set dst (ls src) (undef_regs ml ls)) e.
+  satisf rs (Locmap.set dst (ls @ src) (undef_regs ml ls)) e.
 Proof.
   intros; red; intros.
   exploit in_subst_loc; eauto. intros [[A B] | [A B]].
@@ -1356,7 +1356,7 @@ Lemma return_regs_agree_callee_save:
   forall caller callee,
   agree_callee_save caller (return_regs caller callee).
 Proof.
-  intros; red; intros. unfold return_regs. red in H.
+  intros; red; intros. unfold Locmap.get, return_regs. red in H.
   destruct l.
   rewrite H; auto.
   destruct sl; auto || congruence.
@@ -1483,9 +1483,9 @@ Proof.
   red; intros. rewrite Regmap.gsspec. destruct (peq (ereg q) r1).
   exploit compat_left2_sound; eauto.
   intros [[A B] | [A B]]; rewrite A; rewrite B; simpl.
-  apply Val.lessdef_trans with (Val.hiword (Val.longofwords (ls l1) (ls l2))).
+  apply Val.lessdef_trans with (Val.hiword (Val.longofwords (ls @ l1) (ls @ l2))).
   apply Val.hiword_lessdef; auto. apply val_hiword_longofwords.
-  apply Val.lessdef_trans with (Val.loword (Val.longofwords (ls l1) (ls l2))).
+  apply Val.lessdef_trans with (Val.loword (Val.longofwords (ls @ l1) (ls @ l2))).
   apply Val.loword_lessdef; auto. apply val_loword_longofwords.
   eapply IHb; eauto.
 - (* error case *)
@@ -1499,7 +1499,7 @@ Lemma call_regs_param_values:
 Proof.
   intros. unfold loc_parameters. rewrite list_map_compose.
   apply list_map_exten; intros. symmetry.
-  assert (A: forall l, loc_argument_acceptable l -> call_regs ls (parameter_of_argument l) = ls l).
+  assert (A: forall l, loc_argument_acceptable l -> (call_regs ls) @ (parameter_of_argument l) = ls @ l).
   { destruct l as [r | [] ofs ty]; simpl; auto; contradiction. }
   exploit loc_arguments_acceptable; eauto. destruct x; simpl; intros.
 - auto.
@@ -1517,6 +1517,7 @@ Proof.
   apply list_map_exten; intros.
   apply Locmap.getpair_exten; intros.
   assert (In l (regs_of_rpairs (loc_arguments sg))) by (eapply in_regs_of_rpairs; eauto).
+  unfold Locmap.get.
   exploit loc_arguments_acceptable_2; eauto. exploit H; eauto.
   destruct l; simpl; intros; try contradiction. rewrite H4; auto.
 Qed.
@@ -1528,7 +1529,7 @@ Lemma find_function_tailcall:
 Proof.
   unfold ros_compatible_tailcall, find_function; intros.
   destruct ros as [r|id]; auto.
-  unfold return_regs. destruct (is_callee_save r). discriminate. auto.
+  unfold Locmap.get, return_regs. destruct (is_callee_save r). discriminate. auto.
 Qed.
 
 Lemma loadv_int64_split:
@@ -1564,15 +1565,15 @@ Lemma add_equations_builtin_arg_lessdef:
   add_equations_builtin_arg env arg arg' e = Some e' ->
   satisf rs ls e' ->
   wt_regset env rs ->
-  exists v', eval_builtin_arg ge ls sp m arg' v' /\ Val.lessdef v v'.
+  exists v', eval_builtin_arg ge (Locmap.read ls) sp m arg' v' /\ Val.lessdef v v'.
 Proof.
   induction 1; simpl; intros e e' arg' AE SAT WT; destruct arg'; MonadInv.
 - exploit add_equation_lessdef; eauto. simpl; intros.
-  exists (ls x0); auto with barg.
+  exists (ls @ x0); econstructor; auto with barg; econstructor.
 - destruct arg'1; MonadInv. destruct arg'2; MonadInv.
   exploit add_equation_lessdef. eauto. simpl; intros LD1.
   exploit add_equation_lessdef. eapply add_equation_satisf. eauto. simpl; intros LD2.
-  exists (Val.longofwords (ls x0) (ls x1)); split; auto with barg.
+  exists (Val.longofwords (ls @ x0) (ls @ x1)); split; auto with barg. econstructor; econstructor.
   rewrite <- (val_longofwords_eq_2 rs#x); auto. apply Val.longofwords_lessdef; auto.
   rewrite <- e0; apply WT.
 - econstructor; eauto with barg.
@@ -1610,14 +1611,14 @@ Lemma add_equations_builtin_args_lessdef:
   satisf rs ls e' ->
   wt_regset env rs ->
   Mem.extends m tm ->
-  exists vl', eval_builtin_args ge ls sp tm arg' vl' /\ Val.lessdef_list vl vl'.
+  exists vl', eval_builtin_args ge (Locmap.read ls) sp tm arg' vl' /\ Val.lessdef_list vl vl'.
 Proof.
   induction 1; simpl; intros; destruct arg'; MonadInv.
 - exists (@nil val); split; constructor.
 - exploit IHlist_forall2; eauto. intros (vl' & A & B).
   exploit add_equations_builtin_arg_lessdef; eauto.
   eapply add_equations_builtin_args_satisf; eauto. intros (v1' & C & D).
-  exploit (@eval_builtin_arg_lessdef _ ge ls ls); eauto. intros (v1'' & E & F).
+  exploit (@eval_builtin_arg_lessdef _ ge (Locmap.read ls) (Locmap.read ls)); eauto. intros (v1'' & E & F).
   exists (v1'' :: vl'); split; constructor; auto. eapply Val.lessdef_trans; eauto.
 Qed.
 
@@ -1639,7 +1640,7 @@ Lemma add_equations_debug_args_eval:
   satisf rs ls e' ->
   wt_regset env rs ->
   Mem.extends m tm ->
-  exists vl', eval_builtin_args ge ls sp tm arg' vl'.
+  exists vl', eval_builtin_args ge (Locmap.read ls) sp tm arg' vl'.
 Proof.
   induction 1; simpl; intros; destruct arg'; MonadInv.
 - exists (@nil val); constructor.
@@ -1648,7 +1649,7 @@ Proof.
 + exploit IHlist_forall2; eauto. intros (vl' & B).
   exploit add_equations_builtin_arg_lessdef; eauto.
   eapply add_equations_debug_args_satisf; eauto. intros (v1' & C & D).
-  exploit (@eval_builtin_arg_lessdef _ ge ls ls); eauto. intros (v1'' & E & F).
+  exploit (@eval_builtin_arg_lessdef _ ge (Locmap.read ls) (Locmap.read ls)); eauto. intros (v1'' & E & F).
   exists (v1'' :: vl'); constructor; auto.
 + eauto.
 Qed.
@@ -1666,7 +1667,7 @@ Lemma add_equations_builtin_eval:
   external_call ef ge vargs m1 t vres m2 ->
   satisf rs ls e1 /\
   exists vargs' vres' m2',
-     eval_builtin_args ge ls sp m1' args' vargs'
+     eval_builtin_args ge (Locmap.read ls) sp m1' args' vargs'
   /\ external_call ef ge vargs' m1' t vres' m2'
   /\ Val.lessdef vres vres'
   /\ Mem.extends m2 m2'.
@@ -1675,7 +1676,7 @@ Proof.
   assert (DEFAULT: add_equations_builtin_args env args args' e1 = Some e2 ->
     satisf rs ls e1 /\
     exists vargs' vres' m2',
-       eval_builtin_args ge ls sp m1' args' vargs'
+       eval_builtin_args ge (Locmap.read ls) sp m1' args' vargs'
     /\ external_call ef ge vargs' m1' t vres' m2'
     /\ Val.lessdef vres vres'
     /\ Mem.extends m2 m2').
@@ -1915,7 +1916,7 @@ Opaque destroyed_by_op.
   econstructor. simpl. eauto. auto. auto.
 * (* reg->stack *)
   exploit IHmv; eauto. eapply subst_loc_undef_satisf; eauto.
-  InvBooleans. split; eauto. apply wt_setstack, wt_undef_regs. auto.
+ InvBooleans. split; eauto. apply wt_setstack, wt_undef_regs. auto.
   intros [ls' [A B]]. exists ls'; split; auto. eapply star_left; eauto.
   econstructor. simpl. eauto. auto.
 * (* stack->reg *)
@@ -1928,34 +1929,34 @@ Opaque destroyed_by_op.
 * (* stack->stack *)
   inv H0. simpl in H8. contradiction.
 + (* makelong *)
-  assert (HT: Val.has_type (Val.longofwords (ls (R src1)) (ls (R src2))) (mreg_type dst)).
+  assert (HT: Val.has_type (Val.longofwords (ls @ (R src1)) (ls @ (R src2))) (mreg_type dst)).
   {
     destruct H3; InvBooleans. simpl in H6.
     destruct (mreg_type dst) eqn:T; simpl; auto; inversion H6.
-    destruct (ls (R src1)), (ls (R src2)); simpl; auto.
-    destruct (ls (R src1)), (ls (R src2)); simpl; auto.
+    destruct (ls @ (R src1)), (ls @ (R src2)); simpl; auto.
+    destruct (ls @ (R src1)), (ls @ (R src2)); simpl; auto.
   }
   exploit IHmv; eauto. eapply subst_loc_pair_satisf_makelong; eauto.
   destruct H3; InvBooleans. split; eauto using wt_setreg.
   intros [ls' [A B]]. exists ls'; split; auto. eapply star_left; eauto.
   econstructor. simpl; eauto. reflexivity. traceEq.
 + (* lowlong *)
-  assert (HT: Val.has_type (Val.loword (ls (R src))) (mreg_type dst)).
+  assert (HT: Val.has_type (Val.loword (ls @ (R src))) (mreg_type dst)).
   {
     destruct H3. simpl in H5. InvBooleans.
     destruct (mreg_type dst) eqn:T; simpl; auto; inversion H6;
-      destruct (ls (R src)); simpl; auto.
+      destruct (ls @ (R src)); simpl; auto.
   }
   exploit IHmv; eauto. eapply subst_loc_part_satisf_lowlong; eauto.
   destruct H3; InvBooleans. split; eauto using wt_setreg.
   intros [ls' [A B]]. exists ls'; split; auto. eapply star_left; eauto.
   econstructor. simpl; eauto. reflexivity. traceEq.
 + (* highlong *)
-  assert (HT: Val.has_type (Val.hiword (ls (R src))) (mreg_type dst)).
+  assert (HT: Val.has_type (Val.hiword (ls @ (R src))) (mreg_type dst)).
   {
     destruct H3. simpl in H5. InvBooleans.
     destruct (mreg_type dst) eqn:T; simpl; auto; inversion H6;
-      destruct (ls (R src)); simpl; auto.
+      destruct (ls @ (R src)); simpl; auto.
   }
   exploit IHmv; eauto. eapply subst_loc_part_satisf_highlong; eauto.
   destruct H3; InvBooleans. split; eauto using wt_setreg.
@@ -2532,7 +2533,7 @@ Proof.
   assert (F2': eval_addressing tge sp addr (reglist ls3 args2') = Some a2').
     rewrite <- F2. apply eval_addressing_preserved. exact symbols_preserved.
   exploit (eval_offset_addressing tge); eauto. intros F2''.
-  assert (STOREX: exists m2', Mem.storev Mint32 m1' (Val.add a2' (Vint (Int.repr 4))) (ls3 (R src2')) = Some m2' /\ Mem.extends m' m2').
+  assert (STOREX: exists m2', Mem.storev Mint32 m1' (Val.add a2' (Vint (Int.repr 4))) (ls3 @ (R src2')) = Some m2' /\ Mem.extends m' m2').
   { try discriminate;
     (eapply Mem.storev_extends;
      [eexact EXT1 | eexact STORE2 | apply Val.add_lessdef; [eexact G2|eauto] | eauto]). }
@@ -2683,7 +2684,7 @@ Proof.
   split; auto.
   eapply wt_function_wt_bblock; eauto.
   intros [ls1 [A1 [B1 C1]]].
-  assert (Val.lessdef (Vint n) (ls1 (R arg'))).
+  assert (Val.lessdef (Vint n) (ls1 @ (R arg'))).
     rewrite <- H0. eapply add_equation_lessdef with (q := Eq Full arg (R arg')); eauto.
   inv H2.
   econstructor; split.
@@ -2733,8 +2734,8 @@ Proof.
   rewrite H13. apply WTRS.
   generalize (loc_result_caller_save (RTL.fn_sig f)).
   destruct (loc_result (RTL.fn_sig f)); simpl.
-  intros A; rewrite A; auto.
-  intros [A B]; rewrite A, B; auto.
+  unfold Locmap.get, return_regs. intros A; rewrite A; auto.
+  unfold Locmap.get, return_regs. intros [A B]; rewrite A, B; auto.
   apply return_regs_agree_callee_save.
   unfold proj_sig_res. rewrite <- H11; rewrite H13. apply WTRS.
 
@@ -2787,7 +2788,7 @@ Proof.
   eapply Val.has_subtype; eauto. destruct v'; simpl; auto.
   red; intros. rewrite (AG l H0).
   rewrite locmap_get_set_loc_result_callee_save by auto.
-  unfold undef_caller_save_regs. destruct l; simpl in H0.
+  unfold Locmap.get, undef_caller_save_regs. destruct l; simpl in H0.
   rewrite H0; auto.
   destruct sl; auto; congruence.
   eapply external_call_well_typed; eauto.
