backend/Debugvarproof.v
@@ -344,7 +344,7 @@ Qed.
 
 Lemma can_eval_safe_arg:
   forall (rs: locset) sp m (a: builtin_arg loc),
-  safe_builtin_arg a -> exists v, eval_builtin_arg tge rs sp m a v.
+  safe_builtin_arg a -> exists v, eval_builtin_arg tge (Locmap.read rs) sp m a v.
 Proof.
   induction a; simpl; intros; try contradiction;
   try (econstructor; now eauto with barg).
