backend/Linearizeproof.v
@@ -516,7 +516,7 @@ Inductive match_states: LTL.state -> Linear.state -> Prop :=
         (STACKS: list_forall2 match_stackframes s ts)
         (TRF: transf_function f = OK tf)
         (REACH: (reachable f)!!pc = true)
-        (ARG: ls (R arg) = Vint n)
+        (ARG: ls @ (R arg) = Vint n)
         (JUMP: list_nth_z tbl (Int.unsigned n) = Some pc),
       match_states (LTL.State s f sp pc (undef_regs destroyed_by_jumptable ls) m)
                    (Linear.State ts tf sp (Ljumptable arg tbl :: c) ls m)
